various changes following some suggestions from the Zulip chat

gluing.lean
@@ -85,9 +85,7 @@ def gl_refine : gluing_data (I × J) X Y :=
     gl.hglue i₁ i₂ x hxi₁ hxi₂,
   ⟩
 
-variable (f : X → Y)
-
-lemma compat_of_refine_of_compat :
+lemma compat_of_refine_of_compat (f : X → Y) :
   compatible gl f →
   compatible (gl_refine _ _ _ _ CJ gl) f :=
 begin
@@ -100,33 +98,32 @@ end refine
 end covers
 
 section open_cover
-
 open topology
 
-variables (I X Y : Type) (TX : topology X) (TY : topology Y)
+variables (I X Y : Type) [topology X] [topology Y]
 
 structure open_cover extends (cover I X) :=
-  (hopen : ∀ (i : I), part i ∈ TX.opens)
+  (hopen : ∀ (i : I), part i ∈ topology.opens X)
 
-instance : has_coe (open_cover I X TX) (cover I X) := ⟨λ U, ⟨U.part, U.hx⟩⟩
+instance : has_coe (open_cover I X) (cover I X) := ⟨λ U, ⟨U.part, U.hx⟩⟩
 
 structure cts_gluing_data :=
-  (U : open_cover I X TX)
+  (U : open_cover I X)
   (f : Π (i : I), (U i) → Y)
   (hglue : ∀ (i j : I) (x : X) (hxi : x ∈ U i) (hxj : x ∈ U j),
     (f i) ⟨x, hxi⟩ = (f j) ⟨x, hxj⟩)
-  (hf : Π (i : I), @cts _ _ (topology.subspace_topology TX (U i)) TY (f i))
+  (hf : Π (i : I), cts (f i))
 
-instance : has_coe (cts_gluing_data I X Y TX TY) (gluing_data I X Y) :=
+instance : has_coe (cts_gluing_data I X Y) (gluing_data I X Y) :=
   ⟨λ gl, ⟨gl.U, gl.f, gl.hglue⟩⟩
 
 variables
-  (U : open_cover I X TX) (gl : cts_gluing_data I X Y TX TY)
+  (U : open_cover I X) (gl : cts_gluing_data I X Y)
   (f g : X → Y)
 
-lemma cts_iff_cts_on_cover (f : X → Y) : cts TX TY f ↔ 
-  Π (i : I), @cts _ _ (topology.subspace_topology TX (U i)) TY
-                      (subtype.restrict f _) :=
+lemma cts_iff_cts_on_cover (f : X → Y) : cts f ↔ 
+  Π (i : I), @cts _ _ (topology.subspace_topology (U i)) _
+                      (subtype.restrict f (U i)) :=
 begin
   split,
   intros hf i, apply pullback_cts_along_inverse_image, exact hf,
@@ -135,79 +132,123 @@ begin
   rw cts_iff_ptwise_cts, intro x,
   obtain ⟨i, hxi⟩ := U.hx x, specialize hfi i,
   rw cts_iff_ptwise_cts at hfi, specialize hfi ⟨x, hxi⟩,
-  rwa cts_at_pt_of_open TX TY f (U i) (U.hopen i) x hxi,
+  rwa cts_at_pt_of_open f (U i) (U.hopen i) x hxi,
 end
 
 -- function compatible with cts gluing data is cts
 -- (mostly equivalent to cts_iff_cts_on_cover)
 lemma cts_of_cts_compat :
-  compatible (gl : gluing_data I X Y) f → cts TX TY f :=
+  compatible (gl : gluing_data I X Y) f → cts f :=
 begin
   intro hf,
-  rw cts_iff_cts_on_cover I X Y TX TY gl.U,
+  rw cts_iff_cts_on_cover I X Y gl.U,
   rw compatible_iff_restrict_eq at hf,
   intro i, specialize hf i, convert gl.hf i,
 end
 
 -- the glued function is continuous! 🎉
-lemma mk_function_cts : cts TX TY (mk_function (gl : gluing_data I X Y)) :=
-  @cts_of_cts_compat I X Y TX TY gl
+lemma mk_function_cts : cts (mk_function (gl : gluing_data I X Y)) :=
+  cts_of_cts_compat I X Y gl
   (mk_function (gl : gluing_data I X Y))
   (mk_compatible ↑gl)
 
-section fiber_bundle
+end open_cover
 
-def res_l {X Y : Type} {A B : set X} (g : A → Y) : A ∩ B → Y :=
-  λ ⟨a, hab⟩, g ⟨a, hab.1⟩
+-- an attempt at doing covers using maps rather than subsets
+section b_cover
 
-def res_r {X Y : Type} {A B : set X} (g : B → Y) : A ∩ B → Y :=
-  λ ⟨a, hab⟩, g ⟨a, hab.2⟩
+structure b_cover (I X : Type) :=
+  (part   : I → Type)
+  (map    : Π {i : I}, (part i) → X)
+  (hx     : ∀ (x : X), ∃ i (u : part i), map u = x)
 
--- collecting the data of a potential bundle
--- (this definition does not assert any actual properties of π)
-structure prebundle :=
-  (base fiber total_space : Type)
-  (TB : topology base)
-  (TF : topology fiber)
-  (TT : topology total_space)
-  (π : total_space → base)
-  (hπ : function.surjective π ∧ cts TT TB π)
+instance b_cover_to_parts (I X : Type) : has_coe_to_fun (b_cover I X) :=
+  {F   := λ _, I → Type,
+   coe := λ U, U.part}
 
--- what it means for trivialize over a subset
-structure trivialize_subset (E : prebundle) (U : set E.base) :=
-  (φ : U × E.fiber → E.π ⁻¹' U)
-  (hφ_homeo : homeo ↑((E.TB : topology U), E.TF) ↑E.TT φ)
-  (hφ_proj : ∀ u v, E.π (φ ⟨u, v⟩) = u)
+def to_fun {I X : Type} (U : b_cover I X) (i : I) : U i → X :=
+  λ x, U.map x
 
--- a fiber bundle together with a choice of trivialization datum
-structure structured_fiber_bundle extends prebundle :=
-  (I : Type)
-  (U : open_cover I base TB)
-  (triv (i : I) : trivialize_subset (to_prebundle) (U i))
+structure b_cover₂ (I X : Type) extends (b_cover I X) :=
+  (part₂   : I → I → Type)
+  (map₂l   : Π {i j : I}, (part₂ i j) → part i)
+  (map₂r   : Π {i j : I}, (part₂ i j) → part j)
+  (compat₂ : Π {i j : I} (u_ij : part₂ i j), 
+             map (map₂l u_ij) = map (map₂r u_ij))
+  (hx₂     : ∀ {i j : I} {u_i : part i} {u_j : part j},
+             map u_i = map u_j ↔
+             ∃ u_ij, map₂l u_ij = u_i ∧ map₂r u_ij = u_j)
 
--- incomplete, but will likely be needed
-def refine_trivializing
-  (E : prebundle) (U : set E.base) (triv : trivialize_subset E U)
-  (U' : set E.base) (hU' : U' ⊆ U) :
-  trivialize_subset E U' := sorry
+-- consistent functions on each part of the cover
+structure b_gluing_data (I X Y : Type) extends (b_cover₂ I X) :=
+  (f  : Π {i : I}, part i → Y)
+  (hglue : ∀ {i j : I} (u : part₂ i j),
+           f (map₂l u) = f (map₂r u))
 
+-- what it means for f : X → Y to be compatible with gluing data
+def b_compatible {I X Y : Type} (gl : b_gluing_data I X Y) (f : X → Y) :=
+  ∀ {i : I} (u : gl.part i), f (gl.map u) = gl.f u
 
-/- from earlier attempt to define fiber bundle, including transition functions
-  (trans (i j : I) : (U i) ∩ (U j) → fiber → fiber)
-  (htrans (i j : I) :
-    (∀ (u : (U i) ∩ (U j)) (v : fiber),
-      let t := (triv i ⟨⟨u, u.2.1⟩, v⟩) in -- ⟨t.val, h : t ∈ π ⁻¹' U i⟩
-      triv_inv j ⟨t.val, begin simp, rw (htriv i).2.2.2 ⟨u, u.2.1⟩ v, exact u.2.2, end⟩
-        = ⟨⟨u, u.2.2⟩, trans i j u v⟩))
+-- existence of compatible function
+-- (uses choice, even though the result is unique)
+def b_mk_function {I X Y : Type} (gl : b_gluing_data I X Y) : X → Y :=
+  λ x, let hi := classical.some_spec (gl.hx x) in
+       let u := classical.some hi in
+       gl.f u
+
+lemma b_mk_compatible {I X Y} (gl : b_gluing_data I X Y) :
+  b_compatible gl (b_mk_function gl) :=
+begin
+  intros i v,
+  let hi := classical.some_spec (gl.hx (gl.map v)),
+  let u := classical.some hi,
+  let hu := classical.some_spec hi, rw gl.hx₂ at hu,
+  change gl.f u = gl.f v,
+  obtain ⟨uij, hl, hr⟩ := hu, change gl.map₂l uij = u at hl,
+  have key := gl.hglue uij, rwa [hl, hr] at key,
+end
+
+lemma b_compatible_unique {I X Y : Type} (gl : b_gluing_data I X Y) (f g : X → Y) :
+  b_compatible gl f → b_compatible gl g → f = g :=
+begin
+  intros hf hg,
+  ext, obtain ⟨i, ⟨u, hu⟩⟩ := gl.hx x,
+  specialize hf u, specialize hg u, rw hu at *,
+  rwa [hf, hg],
+end
+
+section b_refine
+
+variables
+  (I J X Y : Type)
+  (CI : b_cover I X)
+  (CJ : b_cover J X)
+  (gl : b_gluing_data I X Y)
+
+def b_refine : b_cover (I × J) X :=
+ ⟨λ ⟨i, j⟩, {uv : CI i × CJ j // CI.map uv.fst = CJ.map uv.snd},
+  λ ⟨i, j⟩ ⟨uv, h⟩, CI.map uv.fst,
+  begin
+    intro x,
+    obtain ⟨i, ⟨u, hu⟩⟩ := CI.hx x,
+    obtain ⟨j, ⟨v, hv⟩⟩ := CJ.hx x,
+    use ⟨i, j⟩, use ⟨u, v⟩, rwa [hu, hv],
+  end⟩
+
+/- 
+Note: this is asymmetric: f is defined on Uᵢ ∩ Vⱼ 
+as the restriction of f from Uᵢ, not Vⱼ.
+-/
+def b_gl_refine : b_gluing_data (I × J) X Y := sorry
+/-
+  ⟨ -- U, f, hglue
+    b_refine I J X CI CJ, -- U
+    λ ⟨i, j⟩ ⟨x, hxij⟩,
+    gl.f i ⟨x, hxij.left⟩,
+    λ ⟨i₁, j₁⟩ ⟨i₂, j₂⟩ x ⟨hxi₁, hxj₁⟩ ⟨hxi₂, hxj₂⟩,
+    gl.hglue i₁ i₂ x hxi₁ hxi₂,
+  ⟩
 -/
 
-
--- This was hard to write -- describing the transition functions especially.
--- It's annoying to have to coerce between different sets.
--- I'm not even sure it's complete.
--- Eventually it will need the transition function to be a rescaling.
-
-
-end fiber_bundle
-
-end open_cover
+end b_refine
+end b_cover
